completion of alpha/beta lemmas

src/etv/alpha_beta.lean
@@ -20,7 +20,7 @@ def is_alpha_cup (a : α) (c : list α) : Prop :=
 instance decidable_is_alpha_cup (a : α) (c : list α) :
   decidable (l.is_alpha_cup a c) := by rw is_alpha_cup; apply_instance
 
-theorem alpha_cup_is_cup {c : list α} 
+theorem alpha_cup_is_cup (c : list α)
   (c_in_S : c.in S) (c_sorted : c.sorted (<))
   (c_chain : c.chain' l.slopeᶜ) : C.cup c :=
 begin
@@ -102,7 +102,8 @@ theorem add_alpha {a : α} (ha : a ∈ S)
 begin
   rcases (l.alpha_cup ha) with 
     ⟨d, d_length, d_in_S, d_sorted, d_chain, d_last⟩,
-  have d_cup : C.cup d := l.alpha_cup_is_cup d_in_S d_sorted d_chain,
+  have d_cup : C.cup d := l.alpha_cup_is_cup 
+   _ d_in_S d_sorted d_chain,
   rcases list.take_last' d_last with ⟨d', eq_d⟩,
   rcases list.take_head' c_head with ⟨c', eq_c⟩,
   use d' ++ a :: c', 
@@ -142,64 +143,133 @@ end config.label
 
 namespace config
 
-variable (C)
+variables (C) (S)
 
-def is_beta_cup {a : α} (ha : a ∈ S) (c : list α) : Prop :=
-  C.cup c ∧ c.last' = some a
+def is_beta_cup (a : α) (c : list α) : Prop :=
+  (c ++ [a]).in S ∧ C.cup (c ++ [a])
 
-instance decidable_is_beta_cup {a : α} (ha : a ∈ S) (c : list α) :
-  decidable (C.is_beta_cup ha c) := by rw is_beta_cup; apply_instance
+instance decidable_is_beta_cup (a : α) (c : list α) :
+  decidable (C.is_beta_cup S a c) := by rw is_beta_cup; apply_instance
 
-def beta_cups {a : α} (ha : a ∈ S) : list (list α) :=
-  (S.sort (≤)).sublists.filter (C.is_beta_cup ha)
+def beta_cups' (a : α) : list (list α) :=
+  (S.sort (≤)).sublists.filter (C.is_beta_cup S a)
 
-def beta_cups_nnil {a : α} (ha : a ∈ S) : C.beta_cups ha ≠ [] :=
-  by apply mem_imply_nnil [a]; simp [beta_cups, is_beta_cup]; tauto
+def beta_cup' (a : α) : option (list α) :=
+  (C.beta_cups' S a).argmax list.length
 
-def beta_cup' {a : α} (ha : a ∈ S) : option (list α) :=
-  (C.beta_cups ha).argmax list.length
-
-def beta_cup'_is_some {a : α} (ha : a ∈ S) : option.is_some (C.beta_cup' ha) :=
+def beta_cup'_is_some {a : α} (ha : a ∈ S) : 
+  option.is_some (C.beta_cup' S a) :=
 begin
   rw ←option.ne_none_iff_is_some, rw config.beta_cup', simp,
-  exact C.beta_cups_nnil ha,
+  apply mem_imply_nnil [], simp [is_beta_cup, beta_cups'], exact ha,
 end
 
-def beta_cup {a : α} (ha : a ∈ S) : list α :=
-  option.get (C.beta_cup'_is_some ha)
+-- one off from actual definition
+def beta (a : α) : ℕ := 
+  if ha : a ∈ S then (option.get (C.beta_cup'_is_some S ha)).length else 0
 
-variable (S)
-
-def beta (a : α) : ℕ :=
-  if ha : a ∈ S then (C.beta_cup ha).length else 0
-
-lemma exists_beta_cup {a : α} (ha : a ∈ S) {n : ℕ} (hn : n ≤ C.beta S a): 
-  ∃ c : list α, C.ncup n c ∧ c.in S ∧ a ∈ c.last' :=
+-- APIs for beta: First, existence of a cup with length alpha + 1
+def beta_cup {a : α} (ha : a ∈ S) : 
+  Σ' c : list α, c.length = C.beta S a + 1 ∧ 
+    c.in S ∧ C.cup c ∧ a ∈ c.last' :=
 begin
-  sorry
+  have some := C.beta_cup'_is_some S ha,
+  set c := option.get some with def_c, 
+  rw beta, rw dif_pos ha, rw ←def_c,
+  have h_argmax := option.get_mem some, 
+  rw [←def_c, beta_cup'] at h_argmax,
+  have c_beta_cup := list.argmax_mem h_argmax,
+  simp [beta_cups', is_beta_cup] at c_beta_cup,
+  use (c ++ [a]), simp, tauto,
 end
 
-/-
-Define a map from delta to some set
-Show that it is injective...
-
-theorem alpha_le_beta : l.alpha a ≤ C.beta S a := sorry
-
-theorem alpha_append_cup
-  {n : ℕ} {c : list α} (hc : C.ncup n c) 
-  (c_in_S : c.in S) (c_head : a ∈ c.head') :
-  C.has_ncup (n + l.alpha a) S := sorry
-
-theorem ff_inc_alpha {a b : α} (sab : ¬l.slope a b)
-  (ha : a ∈ S) (hb : b ∈ S) (a_le_b : a < b) : 
-  l.alpha a < l.alpha b := sorry
-
-theorem tt_inc_alpha {a b : α} (sab : l.slope a b)
-  (ha : a ∈ S) (hb : b ∈ S) (a_le_b : a < b) : 
-  C.beta S a < C.beta S b := sorry
-
-theorem has_beta_cup {a : α} (ha : a ∈ S) : 
-  C.has_ncup (C.beta S a) S := sorry
--/
+-- Next, maximality of the cup with length alpha + 1
+def cup_length_le_beta {a : α} {c : list α}
+  (c_in_S : c.in S) 
+  (c_cup : C.cup c)
+  (c_last : a ∈ c.last') : c.length ≤ C.beta S a + 1 :=
+begin
+  have ha : a ∈ S := c_in_S _ (list.mem_of_mem_last' c_last),
+  have some := C.beta_cup'_is_some S ha,
+  set d := option.get some with def_d, 
+  rw beta, rw dif_pos ha, rw ←def_d,
+  have h_argmax := option.get_mem some, 
+  rw [←def_d, beta_cup'] at h_argmax,
+  rcases list.take_last' c_last with ⟨c', eq_c⟩,
+  subst eq_c, simp,
+  have c_sorted := list.chain'_iff_pairwise.mp c_cup.left,
+  have c'_beta_cup : c' ∈ C.beta_cups' S a := begin
+    rw beta_cups', simp, split,
+    { apply list.sublist_of_subperm_of_sorted _ _ 
+        (finset.sort_sorted_lt S),
+      apply list.nodup.subperm,
+      apply @list.nodup.sublist _ _ (c' ++ [a]), simp,
+      exact (list.sorted.nodup c_sorted),
+      intros a ha, simp, simp at c_in_S, exact (c_in_S.left) _ ha,
+      apply list.pairwise.sublist _ c_sorted, simp, },
+    { split; assumption },
+  end,
+  exact list.le_of_mem_argmax c'_beta_cup h_argmax,
+end
 
 end config
+
+theorem config.label.alpha_le_beta {a : α} (ha : a ∈ S) : 
+  l.alpha a ≤ C.beta S a :=
+begin
+  rcases (l.alpha_cup ha) with 
+    ⟨c, c_length, c_in, c_sorted, c_chain, c_last⟩,
+  have c_cup := l.alpha_cup_is_cup _ c_in c_sorted c_chain,
+  have ineq := C.cup_length_le_beta S c_in c_cup c_last,
+  rw c_length at ineq, simp at ineq, exact ineq,
+end
+
+theorem config.has_beta_cup {a : α} (ha : a ∈ S) :
+  C.has_ncup (C.beta S a + 1) S :=
+begin
+  rcases (C.beta_cup S ha) with 
+    ⟨c, c_length, c_in, c_cup, c_last⟩,
+  use c, rw config.ncup, tauto,
+end
+
+theorem config.label.slope.ff_inc_alpha 
+  {a b : α} (sab : ¬l.slope a b)
+  (ha : a ∈ S) (hb : b ∈ S) (a_le_b : a < b) : 
+  l.alpha a < l.alpha b :=
+begin
+  rcases (l.alpha_cup ha) with 
+    ⟨c, c_length, c_in, c_sorted, c_chain, c_last⟩,
+  rcases list.take_last' c_last with ⟨c', c_eq⟩,
+  rw [nat.lt_iff_add_one_le, ←(add_le_add_iff_right 1)],
+  set d := c ++ [b] with def_d,
+  have d_length : d.length = l.alpha a + 1 + 1 :=
+    by simp [def_d, c_length],
+  rw ←d_length,
+  apply l.cup_length_le_alpha,
+  { rw def_d, simp, tauto, },
+  { rw [def_d, c_eq, list.sorted, ←list.chain'_iff_pairwise], 
+    simp, rw [list.chain'_iff_pairwise, ←list.sorted],
+    rw ←c_eq, exact ⟨c_sorted, a_le_b⟩, },
+  { rw [def_d, c_eq], simp, rw ←c_eq,
+    exact ⟨c_chain, sab⟩, },
+  { rw def_d, simp, },
+end
+
+theorem config.label.slope.tt_inc_beta
+  {a b : α} (sab : l.slope a b)
+  (ha : a ∈ S) (hb : b ∈ S) (a_le_b : a < b) : 
+  C.beta S a < C.beta S b :=
+begin
+  rcases (C.beta_cup S ha) with 
+    ⟨c, c_length, c_in, c_cup, c_last⟩,
+  rcases list.take_last' c_last with ⟨c', c_eq⟩,
+  rw [nat.lt_iff_add_one_le, ←(add_le_add_iff_right 1)],
+  set d := c ++ [b] with def_d,
+  have d_length : d.length = C.beta S a + 1 + 1 :=
+    by simp [def_d, c_length],
+  rw ←d_length,
+  apply C.cup_length_le_beta S; rw def_d,
+  simp, split; assumption,
+  apply c_cup.extend_right sab; try {simp}; try {assumption},
+  simp,
+end
